pprint/Rendering_old.v
@@ -1,0 +1,132 @@
+From Coq Require Import Strings.String.
+From Coq Require Import Strings.Ascii.
+From PPrint Require Import Documents.
+
+(** * Backends. *)
+
+(** The rendering engine does not output strings directly : it is parametric over
+    a backend, which provides a low-level output interface.
+   
+    The job of the backend is to :
+    - accumulate characters and strings ([add_string]).
+    - deal with annotations ([enter_annot], [exit_annot]). 
+
+    I chose to represent a backend as a simple state machine :
+    - [initial_state] is the initial state.
+    - various functions such as [add_char] or [enter_annot] modify the state.
+    - [get_output] extracts the actual output (usually a string) from the state.
+    This representation is simple yet seems to be general enough in practice.
+    
+    Annotations can be nested. For instance :
+      [enter_annot A1 ; add_string "hello" ; enter_annot A2 ; add_string "world" ; exit_annot A2 ; exit_annot A1]
+    will print "hello" with annotation [A1] followed by "world" with annotation [A2].
+    Calls to [enter_annot]/[exit_annot] are always well-parenthesized.
+*)
+Module Type Backend.
+
+(** The output type of this backend. 
+    Usually this is [string], but it could also be some kind of HTML data-structure. *)
+Parameter output : Type.
+
+(** The type of annotations supported by this backend.
+    Basic examples could be :
+    - [Inductive annot := Bold | Italic | Underline.] to support bold, italic or underlined text.
+    - [Record annot := { red : nat ; green : nat ; blue : nat}.] to add color to your text. 
+*)
+Parameter annot : Type.
+
+(** The internal state maintainted by the backend. 
+    This is implementation-specific. *)
+Parameter state : Type.
+  
+(** The initial state. *)
+Parameter init_state : state.
+
+(** Extract the output from a state. *)
+Parameter get_output : state -> output.
+
+(** Add a string. *)
+Parameter add_string : string -> state -> state.
+
+(** Enter an annotation : all characters and strings added between [enter_annot] and 
+    the matching [exit_annot] should have the annotation [annot] applied to them. *)
+Parameter enter_annot : annot -> state -> state.
+
+(** Exit an annotation. The [annot] argument is the same as in the corresponding [enter_annot]. *)
+Parameter exit_annot : annot -> state -> state.
+  
+End Backend.
+  
+(** * Rendering a document to a backend. *)
+
+(** The rendering engine is parametric over a backend. *)
+Module Make (B : Backend).
+
+(** [make_string n c] makes a string of length [n] filled with the character [c]. *)
+Definition make_string (n : nat) (c : Ascii.ascii) : string :=
+  let fix loop n acc :=
+    match n with 
+    | 0 => acc
+    | S n => loop n (String c acc)
+    end
+  in 
+  loop n EmptyString.
+
+(** [pretty doc flat width indent col st] is the main function in the rendering engine :
+    - [doc] is the document we are printing.
+    - [flat] is [true] if we are in flat mode, otherwise it is [false].
+    - [width] is the maximum character width we are allowed to use.
+    - [indent] is the current indentation level : [indent] blank characters are added after each newline.
+    - [col] is the current column index, starting at 0.
+    - [st] is the backend state.
+
+    As documents can become quite big, we are careful to write this function in tail-recursive style.
+    The continuation is passed : 
+    - the resulting column index.
+    - the resulting backend state.
+*)
+Fixpoint pretty {T} (doc : doc B.annot) (flat : bool) (width indent col : nat) (state : B.state) (k : nat -> B.state -> T) : T :=
+  match doc with
+  | Empty => k col state
+  | Str len s => k (col + len) (B.add_string s state)
+  | Blank n => k (col + n) (B.add_string (make_string n " "%char) state)
+  | HardLine =>
+      (* We should be in normal mode here. *)
+      let state := B.add_string (make_string 1 "010"%char) state in
+      let state := B.add_string (make_string indent " "%char) state in
+      k indent state
+  | IfFlat doc1 doc2 =>
+      (* Print [doc1] or [doc2] depending on the current mode. *)
+      pretty (if flat then doc1 else doc2) flat width indent col state k
+  | Cat _ doc1 doc2 =>
+      (* Print [doc1] followed by [doc2]. *)
+      pretty doc1 flat width indent col state (fun col state =>
+        pretty doc2 flat width indent col state k)
+  | Nest _ n doc => 
+      (* Simply increase the indentation amount. *)
+      pretty doc flat width (indent + n) col state k
+  | Group req doc =>
+      (* Determine if [doc] should be flattened. *)
+      let doc_flat := 
+        match req with 
+        | Width req => Nat.leb (col + req) width
+        | Infinity => false
+        end
+      in
+      (* Take care to stay in flattening mode if we are already in it. *)
+      pretty doc (flat || doc_flat) width indent col state k
+  | Align _ doc => 
+      (* Set the indentation amount to the current column. *)
+      pretty doc flat width col col state k
+  | Annot _ ann doc =>
+      let state := B.enter_annot ann state in
+      pretty doc flat width indent col state (fun col state =>
+        let state := B.exit_annot ann state in k col state)
+  end.
+
+(** [pp width doc] pretty-prints the document [doc] to the backend,
+    using a maximum character width of [width]. *)
+Definition pp `{width : nat} doc : B.output :=
+  pretty doc false width 0 0 B.init_state (fun _ state => B.get_output state).
+
+End Make.
